some rewriting

Combi.v
@@ -28,7 +28,7 @@ Fixpoint comparet t : tot t -> tot t -> Prop :=
     fun f g =>
       let it1 := interp t1 in
       let it2 := interp t2 in
-      ((Fun it1 it2) f /\ (Fun it1 it2) g) /\
+      (((Fun it1 it2) f /\ (Fun it1 it2) g)) /\
       forall x, it1 x -> comparet t2 (f x) (g x)
   end
 with interp t: Ensemble (tot t) :=
@@ -51,8 +51,8 @@ Proof.
   - simpl; intros.
     decompose [and] H.
     intuition.
-    specialize H4 with x0.
-    specialize H7 with x0.
+    specialize H5 with x0.
+    specialize H6 with x0.
     specialize IHt2 with (x x0) (y x0) (z x0).
     intuition.
 Qed.
@@ -67,7 +67,7 @@ Fixpoint plus (t:type) : tot t -> nat -> tot t :=
 Lemma plus_arr t1 t2 : plus (Arrow t1 t2) = fun f k x => plus t2 (f x) k.
 Proof. auto. Qed.
 
-Lemma in_interp_arrow t1 t2 v : interp (Arrow t1 t2) v ->forall x, interp t1 x -> interp t2 (v x).
+Lemma in_interp_arrow {t1 t2 v} : forall x, interp (Arrow t1 t2) v -> interp t1 x -> interp t2 (v x).
 Proof.
   intros.
   simpl in H.
@@ -79,72 +79,64 @@ Qed.
 
 Require Import Lia.
 
-Lemma prop_2 (t:type) :
-  (forall x, interp t x -> forall k, interp t (plus t x k))
-  /\ (forall v1 v2, interp t v1 -> interp t v2 ->
-    comparet t v1 v2 -> forall k, comparet t (plus t v1 k) (plus t v2 k)).
+Definition Plus_well_def (t:type) := forall x k, interp t x -> interp t (plus t x k).
+
+Definition Compare_compat_plus (t:type) :=
+  forall v1 v2 k,
+    interp t v1 -> interp t v2 ->
+    comparet t v1 v2 -> comparet t (plus t v1 k) (plus t v2 k).
+
+Lemma prop_2 (t:type) : Plus_well_def t /\ Compare_compat_plus t.
 Proof.
+  unfold Plus_well_def; unfold Compare_compat_plus.
   induction t.
   - split.
     + intros.
       exact (Full_intro nat (x+k)).
     + intros; simpl. unfold comparet in H1.
       lia.
-  - destruct IHt1.
-    destruct IHt2.
+  - destruct IHt1 as (PWDt1,CPTt1).
+    destruct IHt2 as (PWDt2,CPTt2).
     split.
     + intros.
-      rewrite plus_arr.
-      fold tot.
+      rewrite plus_arr; fold tot.
       simpl.
-      simpl in H3.
-      destruct H3.
       split.
       * unfold Fun.
         intros.
-        apply (H3 x0) in H5.
-        exact (H1 (x x0) H5 k).
+        apply PWDt2.
+        exact (in_interp_arrow x0 H H0).
       * intros.
-        specialize H2 with (x v1) (x v2) k.
-        specialize H4 with v1 v2.
-        pose (H31 := H3 v1 H5).
-        pose (H32 := H3 v2 H6).
-        pose (FH := H4 H5 H6 H7).
-        exact (H2 H31 H32 FH).
+        apply (CPTt2 (x v1) (x v2) k (in_interp_arrow v1 H H0) (in_interp_arrow v2 H H1)).
+        simpl in H.
+        destruct H as (_,H).
+        intuition.
     + intros; simpl; intros.
       fold tot.
-      simpl in H5.
-      decompose [and] H5.
-      repeat split.
-      * unfold Fun.
-        intros.
-        unfold Fun in H6.
-        specialize H6 with x.
-        apply H6 in H7.
-        exact (H1 (v1 x) H7 k).
-      * unfold Fun.
-        intros.
-        unfold Fun in H8.
-        specialize H8 with x.
-        apply H8 in H7.
-        exact (H1 (v2 x) H7 k).
+      split.
+      * split.
+        ** unfold Fun.
+           intros.
+           apply PWDt2.
+           exact (in_interp_arrow x H H2).
+        ** unfold Fun.
+           intros.
+           apply PWDt2.
+           exact (in_interp_arrow x H0 H2).
       * intros.
-        specialize H2 with (v1 x) (v2 x) k.
-        apply H2.
-        apply in_interp_arrow. intuition. intuition.
-        apply in_interp_arrow. intuition. intuition.
+        apply CPTt2.
+        exact (in_interp_arrow x H H2).
+        exact (in_interp_arrow x H0 H2).
+        simpl in H1.
         intuition.
 Qed.
 
-Lemma plus_well_def (t:type) :
-  (forall x, interp t x -> forall k, interp t (plus t x k)).
+Lemma plus_well_def (t:type) : Plus_well_def t.
 Proof.
   exact (proj1 (prop_2 t)).
 Qed.
 
-Lemma compare_compat_plus (t:type) :
-  (forall v1 v2, interp t v1 -> interp t v2 ->
-    comparet t v1 v2 -> forall k, comparet t (plus t v1 k) (plus t v2 k)).
+Lemma compare_compat_plus (t:type) : Compare_compat_plus t.
 Proof.
   exact (proj2 (prop_2 t)).
 Qed.
@@ -232,24 +224,24 @@ Proof.
       * intros.
         specialize H0 with v1 v2.
         apply compare_plus_H.
-        exact (H0 H3 H4 H5).
+        exact H1.
+        intuition.
     + intros.
       simpl.
+      apply H2.
+      exact (in_interp_arrow (star t1) H3 H).
+      exact (in_interp_arrow (star t1) H4 H).
       simpl in H5.
-      specialize H5 with (star t1).
-      pose (H3x := in_interp_arrow H3 (star t1) H).
-      pose (H4x := in_interp_arrow H4 (star t1) H).
-      specialize H2 with (v (star t1)) (v' (star t1)).
-      exact (H2 H3x H4x (H5 H)).
+      intuition.
 Qed.
 
-Lemma star_well_def t : InInterp t (star t).
+Lemma star_well_def t : interp t (star t).
 Proof.
   exact (proj1 (prop_4 t)).
 Qed.
 
 Lemma collapse_spec t: forall v v',
-    InInterp t v -> InInterp t v' -> comparet t v v' ->
+    interp t v -> interp t v' -> comparet t v v' ->
     collapse t v < collapse t v'.
 Proof.
   exact (proj2 (prop_4 t)).
@@ -279,11 +271,3 @@ Fixpoint le_t t : tot t -> tot t -> Prop :=
     fun f g =>
       let compare_t2 := comparet t2 in
       forall x, In (tot t1) (interp t1) x -> le_t t2 (f x) (g x) end.
-
-Lemma le_t_refl t : forall x, le_t t x x.
-Proof.
-  induction t.
-  - simpl. exact le_refl.
-  - intros.
-    simpl.
-    intros.
